\documentclass{article}

\input{imports}

\begin{document}

\title{DPP Assignment 2}
\author{Cornelius Sevald-Krause \\ \texttt{<lgx292>}}
\date{2022-12-09}
\maketitle

\section*{Task 1}

\section*{Task 2}

Let $H = (max^s) \times h_2 \times h_3 \times h_4$ where $h_2 , h_3 , h_4$ are
to be determined. We also need to determine $\otimes'_1 , \otimes'_2 ,
\otimes'_3$ and $\otimes'_4$.

First we need to show that the following is true:

\begin{equation}\label{eq:max_cross}
    max^s\ (xs \crossop_{+} ys) = max\ xs + max\ ys
\end{equation}
where $max$ is defined as $max^s$ but over lists instead of sets.

\begin{proof}
    From the definition of $\crossop_{\oplus}$ and $max^s$ we have
    \[
        max^s\ \left(
            [x_1, \ldots, x_n] \crossop_{+} [y_1, \ldots, y_m]
        \right) = x_i + y_j
    \]
    where $1 \leq i \leq n$ and $1 \leq j \leq m$ are chosen such that they
    maximize $x_i + y_j$. As maximizing a sum of two numbers is the same as
    maximizing the two individual numbers, we can conclude that
    $x_i = max\ [x_1, \ldots, x_n]$ and $y_j = max\ [y_1, \ldots, y_m]$.
    Substituting $x_i$ and $y_j$ in the formula above we get
    $max^s\ (xs \crossop_{+} ys) = max\ xs + max\ ys$.
\end{proof}

We can now derive $H$ and $\otimes'_1 , \otimes'_2 , \otimes'_3 , \otimes'_4$.
We start with $\otimes'_1$:
\begin{align*}
      & max^s\ ((s_1,i_1,t_1,d_1) \otimes_1 (s_2,i_2,t_2,d_2))          \\
    = & \quad \{\ \text{Def. of $\otimes_1$}\ \}                        \\
      & max^s\ (s_1 \cup s_2 \cup (t_1 \crossop_{+} i_2))                \\
    = & \quad \{\ \text{Def. of $max^s$}\ \}                            \\
      & max^s\ s_1 \maxop mas^s s_2 \maxop max^s\ (t_1 \crossop_{+} i_2) \\
    = & \quad \{\ \eqref{eq:max_cross}\ \}                              \\
      & max^s\ s_1 \maxop mas^s s_2 \maxop max\ t_1 + max\ i_2          \\
\end{align*}
Matching the last part with:
\[
    (max^s\ s_1, h_2\ i_1, h_3\ t_1, h_4\ d_1) \otimes'_1
    (max^s\ s_2, h_2\ i_2, h_3\ t_2, h_4\ d_2)
\]
gives
\begin{align*}
    & h_2 = h_3 = max \\
    & (s_1, i_1, t_1, d_1) \otimes'_1
      (s_2, i_2, t_2, d_2)
    = s_1 \maxop s_2 \maxop (t_1 + i_2)
\end{align*}

We now derive $\otimes'_2$:
\begin{align*}
      & max\ ((s_1,i_1,t_1,d_1) \otimes_2 (s_2,i_2,t_2,d_2))    \\
    = & \quad \{\ \text{Def. of $\otimes_2$}\ \}                \\
      & max\ (i_1 \concat (d_1 +) \map i_2)                     \\
    = & \quad \{\ \text{Def. of $max$}\ \}                      \\
      & max\ i_1 \maxop max\ ((d_1 +) \map i_2)                 \\
    = & \quad \{\ \text{
            $max\ (f \map xs) = f\ (max\ xs)$
            for non-decreasing $f$
        }\ \}                                                   \\
      & max\ i_1 \maxop (d_1 + max\ i_2)                        \\
    = & \quad \{\ \text{Def. of $id$}\ \}                       \\
      & max\ i_1 \maxop (id\ d_1 + max\ i_2)                    \\
\end{align*}
Matching the last part with:
\[
    (max^s\ s_1, h_2\ i_1, h_3\ t_1, h_4\ d_1) \otimes'_2
    (max^s\ s_2, h_2\ i_2, h_3\ t_2, h_4\ d_2)
\]
gives
\begin{align*}
    & h_2 = max \\
    & h_4 = id  \\
    & (s_1, i_1, t_1, d_1) \otimes'_2
      (s_2, i_2, t_2, d_2)
    = i_1 \maxop (d_1 + i_2)
\end{align*}
We have now derived $H = (max^s) \times (max) \times (max) \times (id)$.
We won't show the derivation of $\otimes'_3$ and $\otimes'_4$ but their
definitions are shown below:

\begin{align*}
    (s_1, i_1, t_1, d_1)
    \otimes'_3
    (s_2, i_2, t_2, d_2)
    &= (d_2 + t_1) \maxop t_2   \\
    (s_1, i_1, t_1, d_1)
    \otimes'_4
    (s_2, i_2, t_2, d_2)
    &= d_1 + d_2                \\
\end{align*}

Finally, we show that $h_j \compose f'_j = id$ for $j = 1, \ldots , 4$:
\begin{alignat*}{2}
    (h_1 \compose f_1)\ x &= max^s\ \{ x \} \ &= x \\
    (h_2 \compose f_2)\ x &= max\     [x]   \ &= x \\
    (h_3 \compose f_3)\ x &= max\     [x]   \ &= x \\
    (h_4 \compose f_4)\ x &= id\       x    \ &= x \\
\end{alignat*}

\end{document}
